Scratch2.thy
@@ -1,233 +1,278 @@
 theory Scratch2
-imports Main Rewrite
+imports Main Hoare_Tactics Procs_Typed RHL_Typed
 begin
 
-ML "open Rewrite"
+abbreviation "res == LVariable ''res''"
+abbreviation "args == LVariable ''args''"
 
-lemma 
-  fixes x :: nat
-  assumes x: "x=2"
-  shows "4*4=8"
-  apply (rewrite at 4 eq_reflection)
+lemma rhoare_untypedI: 
+  assumes "\<And>m1 m2. P m1 m2 \<Longrightarrow>
+            (\<exists>\<mu>. apply_to_distr fst \<mu> = denotation_untyped p1 m1 \<and>
+                  apply_to_distr snd \<mu> = denotation_untyped p2 m2 \<and> (\<forall>m1' m2'. (m1',m2') \<in> support_distr \<mu> \<longrightarrow> Q m1' m2'))"
+  shows "rhoare_untyped P p1 p2 Q"
+unfolding rhoare_untyped_rhoare_denotation rhoare_denotation_def using assms by simp
+
+lemma rhoare_untypedE: 
+  assumes "rhoare_untyped P p1 p2 Q"
+  assumes "P m1 m2"
+  shows "\<exists>\<mu>. apply_to_distr fst \<mu> = denotation_untyped p1 m1 \<and>
+                  apply_to_distr snd \<mu> = denotation_untyped p2 m2 \<and> (\<forall>m1' m2'. (m1',m2') \<in> support_distr \<mu> \<longrightarrow> Q m1' m2')"
+using assms unfolding rhoare_untyped_rhoare_denotation rhoare_denotation_def by simp
+
+lemma rhoareI: 
+  assumes "\<And>m1 m2. P m1 m2 \<Longrightarrow>
+            (\<exists>\<mu>. apply_to_distr fst \<mu> = denotation p1 m1 \<and>
+                  apply_to_distr snd \<mu> = denotation p2 m2 \<and> (\<forall>m1' m2'. (m1',m2') \<in> support_distr \<mu> \<longrightarrow> Q m1' m2'))"
+  shows "rhoare P p1 p2 Q"
+unfolding rhoare_def using assms by simp
+
+lemma rhoareE: 
+  assumes "rhoare P p1 p2 Q"
+  assumes "P m1 m2"
+  shows "\<exists>\<mu>. apply_to_distr fst \<mu> = denotation p1 m1 \<and>
+                  apply_to_distr snd \<mu> = denotation p2 m2 \<and> (\<forall>m1' m2'. (m1',m2') \<in> support_distr \<mu> \<longrightarrow> Q m1' m2')"
+using assms unfolding rhoare_def by simp
+
+
+fun list_pattern_untyped :: "variable_untyped list \<Rightarrow> pattern_untyped" where
+  "list_pattern_untyped [] = pattern_ignore unit_type"
+| "list_pattern_untyped (x#xs) = pair_pattern_untyped (pattern_1var x) (list_pattern_untyped xs)"
+
+definition "memory_pattern_related p1 p2 m1 m2 = (\<exists>v. m1 = memory_update_pattern m1 p1 v \<and> m2 = memory_update_pattern m2 p2 v)"
+
+
+definition kill_vars_pattern :: "'a pattern \<Rightarrow> variable_untyped set \<Rightarrow> 'a pattern" where
+  "kill_vars_pattern = undefined"
+
+lemma memory_update_pattern_twice_kill: 
+  "memory_update_pattern (memory_update_pattern m p x) q y = 
+   memory_update_pattern (memory_update_pattern m (kill_vars_pattern p (set (p_vars q))) x) q y"
+  sorry
+
+lemma memory_update_pattern_twice [simp]: "memory_update_pattern (memory_update_pattern m p x) p y = memory_update_pattern m p y"
+  sorry
+
+lemma memory_pattern_relatedI: "m1 = memory_update_pattern m1' p1 v \<Longrightarrow> m2 = memory_update_pattern m2' p2 v \<Longrightarrow> memory_pattern_related p1 p2 m1 m2"
+  unfolding memory_pattern_related_def by auto
+
+(* lemma memory_pattern_related_unit_pattern [simp]: "memory_pattern_related unit_pattern unit_pattern m1 m2"
+  unfolding memory_pattern_related_def memory_update_unit_pattern by auto *)
+
+lemma memory_pattern_related_variable_pattern [simp]: 
+  "memory_pattern_related (variable_pattern x) (variable_pattern y) m1 m2 = (memory_lookup m1 x = memory_lookup m2 y)"
+  unfolding memory_pattern_related_def memory_update_variable_pattern
+  by (metis memory_update_lookup memory_lookup_update_same)
+
+
+lemma memory_update_pattern_swap: "memory_update_pattern (memory_update_pattern m a x) b y
+     = memory_update_pattern (memory_update_pattern m b y) (kill_vars_pattern a (set (p_vars b))) x"
+     sorry
+
+lemma memory_pattern_related_pair_pattern [simp]: 
+  "memory_pattern_related (pair_pattern a1 a2) (pair_pattern b1 b2) m1 m2
+     = (memory_pattern_related a2 b2 m1 m2 
+     \<and> memory_pattern_related (kill_vars_pattern a1 (set (p_vars a2))) (kill_vars_pattern b1 (set (p_vars b2))) m1 m2)" (is "?lhs=?rhs")
+proof (rule iffI)
+  assume "memory_pattern_related (pair_pattern a1 a2) (pair_pattern b1 b2) m1 m2"
+  then obtain a b where m1: "m1 = memory_update_pattern (memory_update_pattern m1 a1 a) a2 b" and
+        m2: "m2 = memory_update_pattern (memory_update_pattern m2 b1 a) b2 b"
+  unfolding memory_pattern_related_def split_paired_Ex memory_update_pair_pattern by auto
+  have "memory_pattern_related a2 b2 m1 m2"
+    apply (rule memory_pattern_relatedI)
+     close (subst m1, rule refl)
+    by (subst m2, rule refl)
+
+  moreover have "memory_pattern_related (kill_vars_pattern a1 (p_vars a2)) (kill_vars_pattern b1 (p_vars b2)) m1 m2"
+    apply (rule memory_pattern_relatedI)
+     apply (subst memory_update_pattern_swap[symmetric])
+     close (subst m1, rule refl)
+    apply (subst memory_update_pattern_swap[symmetric])
+    by (subst m2, rule refl)
+
+  ultimately show "?rhs" by simp
+next
+  assume "?rhs"
+  hence 2: "memory_pattern_related a2 b2 m1 m2" and 1: "memory_pattern_related (kill_vars_pattern a1 (p_vars a2)) (kill_vars_pattern b1 (p_vars b2)) m1 m2"
+    by simp_all
+  from 2 obtain v where m1a2: "m1 = memory_update_pattern m1 a2 v" and m2b2: "m2 = memory_update_pattern m2 b2 v"
+    unfolding memory_pattern_related_def by auto
+  from 1 obtain w where m1a1: "m1 = memory_update_pattern m1 (kill_vars_pattern a1 (p_vars a2)) w" and
+          m2b1: "m2 = memory_update_pattern m2 (kill_vars_pattern b1 (p_vars b2)) w"
+    unfolding memory_pattern_related_def by auto
+  have "m1 = memory_update_pattern m1 (pair_pattern a1 a2) (w,v)"
+    unfolding memory_update_pair_pattern 
+    apply (subst memory_update_pattern_twice_kill[of _ a1 _ a2])
+    apply (subst m1a2) apply (subst m1a1) by simp
+  moreover have "m2 = memory_update_pattern m2 (pair_pattern b1 b2) (w,v)"
+    unfolding memory_update_pair_pattern 
+    apply (subst memory_update_pattern_twice_kill[of _ b1 _ b2])
+    apply (subst m2b2) apply (subst m2b1) by simp
+  ultimately show "memory_pattern_related (pair_pattern a1 a2) (pair_pattern b1 b2) m1 m2"
+    by (rule memory_pattern_relatedI)
+qed
+
+lemma memory_pattern_related_ignore_pattern1 [simp]: 
+  "memory_pattern_related ignore_pattern p m1 m2"
+  sorry
+
+lemma memory_pattern_related_ignore_pattern2 [simp]: 
+  "memory_pattern_related p ignore_pattern m1 m2"
+  sorry
+
+lemma kill_vars_pattern_pair_pattern [simp]: "kill_vars_pattern (pair_pattern p q) V = pair_pattern (kill_vars_pattern p V) (kill_vars_pattern q V)"
+  sorry
+(* lemma kill_vars_pattern_unit_pattern [simp]: "kill_vars_pattern (unit_pattern) V = unit_pattern"
+  sorry *)
+lemma kill_vars_pattern_ignore_pattern [simp]: "kill_vars_pattern (ignore_pattern) V = ignore_pattern"
+  sorry
+lemma kill_vars_pattern_variable_pattern1 [simp]: 
+  "mk_variable_untyped x \<in> V \<Longrightarrow> kill_vars_pattern (variable_pattern x) V = ignore_pattern"
+  sorry
+lemma kill_vars_pattern_variable_pattern2 [simp]: 
+  "mk_variable_untyped x \<notin> V \<Longrightarrow> kill_vars_pattern (variable_pattern x) V = variable_pattern x"
+  sorry
+
+lemma
+  assumes "mk_variable_untyped x \<noteq> mk_variable_untyped y"
+  assumes "mk_variable_untyped y \<noteq> mk_variable_untyped x"
+  assumes "mk_variable_untyped x \<noteq> mk_variable_untyped z"
+  assumes "mk_variable_untyped z \<noteq> mk_variable_untyped x"
+  assumes "mk_variable_untyped z \<noteq> mk_variable_untyped y"
+  assumes "mk_variable_untyped y \<noteq> mk_variable_untyped z"
+  assumes "mk_variable_untyped z \<noteq> mk_variable_untyped a"
+  shows "memory_pattern_related (pair_pattern (variable_pattern x) (pair_pattern (variable_pattern y) (variable_pattern z))) (pair_pattern (variable_pattern z) (pair_pattern (variable_pattern a) ignore_pattern)) m1 m2"
+  apply (auto simp: assms)
+oops
+
+lemma callproc_equiv: 
+  assumes "set (vars_proc_global f) \<subseteq> V1"
+  assumes "V2 \<subseteq> V1"
+  assumes "set (p_vars x1) \<inter> V2 = {}"
+  assumes "set (p_vars x2) \<inter> V2 = {}"
+  shows "rhoare (\<lambda>m1 m2. (\<forall>v\<in>V1. memory_lookup_untyped m1 v = memory_lookup_untyped m2 v)
+                      \<and> e_fun e1 m1 = e_fun e2 m2)
+                   (callproc x1 f e1) (callproc x2 f e2)
+                (\<lambda>m1 m2. (\<forall>v\<in>V2. memory_lookup_untyped m1 v = memory_lookup_untyped m2 v)
+                      \<and> memory_pattern_related x1 x2 m1 m2)"
 proof -
-
-ML_val {*
-  val pat = [At, Term (@{term "4::nat"},[])]
-  val res = rewrite_conv @{context} (pat,NONE) @{thms eq_reflection}
-            @{cterm "4*4=8"}
-*}
-  apply (rewrite at x x)
   
 
+lemma callproc_subst:
+  fixes x1::"'x1::prog_type pattern" and x2::"'x2::prog_type pattern" and y1 y2 and x1e::"'x1 expression" and x2e::"'x2 expression"
+  assumes rhoare: "rhoare P' (callproc x1' f1 y1') (callproc x2' f2 y2') Q'"
+  shows "rhoare P (callproc x1 f1 y1) (callproc x2 f2 y2) Q"
+proof (rule rhoareI, goal_cases)
+case (1 m1 m2)
+  fix in1 in2 (* TODO define *)
+  def m1' == "in1 m1 :: memory" and m2' == "in2 m2 :: memory"
+  have P': "P' m1' m2'" by later
+  obtain \<mu>' where fst': "apply_to_distr fst \<mu>' = denotation (callproc x1' f1 y1') m1'"
+              and snd': "apply_to_distr snd \<mu>' = denotation (callproc x2' f2 y2') m2'"
+              and supp': "\<And>m1'f m2'f. (m1'f,m2'f) \<in> support_distr \<mu>' \<Longrightarrow> Q' m1'f m2'f"
+    apply atomize_elim using P' by (rule rhoare[THEN rhoareE])
+  fix out1 out2 (* TODO define *)
 
+  have Q'_Q: "\<And>x y. Q' x y \<Longrightarrow> Q (out1 x) (out2 y)" by later
+  def \<mu> == "apply_to_distr (\<lambda>(m1f,m2f). (out1 m1f, out2 m2f)) \<mu>' :: (memory\<times>memory) distr"
 
-ML {*
-  val pc0 : Rewrite.patconv = rewrs_pconv NONE @{thms refl}
-  val pc : Rewrite.patconv =  pc0 
-  (* |> (fn p => Rewrite.match_pconv p (@{term "5::int"},[]))  *)
-  |> params_pconv o concl_pconv
-  (* |> in_pconv *)
-;;
-  
-  pc
-  @{context} (Vartab.empty,[]) @{cterm "x*5=x"}
-*}
+  have y1'y1: "e_fun y1' m1' = e_fun y1 m1" by auto
+  have rel1: "denotation (callproc x1 f1 y1) m1 = apply_to_distr out1 (denotation (callproc x1' f1 y1') m1')" 
+    unfolding denotation_callproc y1'y1 Let_def 
+    unfolding apply_to_distr_twice
+    unfolding m1'_def
+    apply (tactic \<open>cong_tac @{context} 1\<close>; (rule refl)?)+
 
+by later
+  hence fst: "apply_to_distr fst \<mu> = denotation (callproc x1 f1 y1) m1" 
+    unfolding \<mu>_def split_def using fst'[THEN arg_cong[where f="apply_to_distr out1"]] by auto
+  have rel2: "denotation (callproc x2 f2 y2) m2 = apply_to_distr out2 (denotation (callproc x2' f2 y2') m2')" by later
+  hence snd: "apply_to_distr snd \<mu> = denotation (callproc x2 f2 y2) m2"
+    unfolding \<mu>_def split_def using snd'[THEN arg_cong[where f="apply_to_distr out2"]] by auto
+  have supp: "\<And>m1f m2f. (m1f,m2f) \<in> support_distr \<mu> \<Longrightarrow> Q m1f m2f" 
+    unfolding \<mu>_def using supp' by (auto intro!: Q'_Q)
+  from fst snd supp show ?case by auto
+qed
 
-ML
-module_type ('pk) EncScheme =
-  keygen :: "(unit,unit) procedure"
+lemma callproc_subst:
+  fixes x1::"'x1::prog_type pattern" and x2::"'x2::prog_type pattern" and y1 y2 and x1e::"'x1 expression" and x2e::"'x2 expression"
+  assumes "rhoare P
+              (callproc (variable_pattern res) f1 (var_expression args))
+              (callproc (variable_pattern res) f2 (var_expression args))
+              Q"
+  defines "P' == \<lambda>m1 m2. P (memory_update m1 args (e_fun y1 m1)) (memory_update m2 args (e_fun y2 m2))"
+  defines "Q' == \<lambda>m1 m2. Q (memory_update m1 res (e_fun x1e m1)) (memory_update m2 res (e_fun x2e m2))"
+  shows "rhoare P' (callproc x1 f1 y1) (callproc x2 f2 y2) Q'"
+proof -
+  (* Proof plan: 
 
-module_type 'a XX = f :: "(unit,unit)procedure"
+  - V=globals \<union> res, arg, footprint
 
-(* declare [[ML_exception_trace]] *)
-ML "open Procs_Typed"
+  - callproc x1=f1(y1)    obseq(V)    "unfolding of it"
+  - callproc x2=f2(y2)    obseq(V)    "unfolding of it"
+  - callproc res=f1(args) obseq(V)    "unfolding of it"
+  - callproc res=f2(args) obseq(V)    "unfolding of it"
 
-local_setup {* fn lthy =>
-  let
-val spec = {name= @{binding X}, procedures=[], type_params=[]}
-val rep_binding = Binding.suffix_name "_rep" (#name spec)
-      val tparams = map fst (#type_params spec)
-      val proctypes = map snd (#procedures spec)
-      val proctypes_tuple = HOLogic.mk_tupleT proctypes
+  - rhoare P (res=f1(args)) ... Q  \<Longrightarrow>  rhoare P (unfold res=f1(args)) ... Q   (uses footprint P,Q in V)
+  - rhoare P (unfold res=f1(args)) ... Q   \<Longrightarrow>   rhoare P' (unfold x1=f1(y1)) ... Q'   (using wp, sp etc)
+  - rhoare P' (unfold x1=f1(y1)) ... Q'  \<Longrightarrow>  rhoare P' (x1=f1(y1)) .. Q'    (footprint P,Q in V)
 
-      val lthy_start = lthy
+  Constraints on V: 
+  - contains all globals
 
-      (* Declaring: type_synonym ('a,'b) ModuleType_rep = "(unit,unit) procedure * (unit,'b) procedure" *)
-      val (rep_type_name,lthy) = Typedecl.abbrev (rep_binding,tparams,NoSyn) proctypes_tuple lthy
-      val rep_type = Type(rep_type_name, map TFree (#type_params spec))
+  *)
+thm callproc_rule
+qed
 
-      (* Declaring: typedef ('a,'b) ModuleType = "UNIV :: ('a::prog_type,'b::prog_type) ModuleType_rep set" *)
-      val typedef_repset = HOLogic.mk_UNIV (rep_type)
-      val ((abs_type_name,typedef_info),lthy) = 
-(* TODO: is overloaded necessary? https://groups.google.com/forum/#!topic/fa.isabelle/Azn3NBvNSgM *)
-          Typedef.add_typedef {overloaded=true} (#name spec, #type_params spec, NoSyn)
-              typedef_repset NONE (fn ctx => (resolve_tac ctx @{thms UNIV_witness} 1)) lthy
-      val abs_type = Type(abs_type_name, map TFree (#type_params spec))
-      (* val Rep_MT = Const(#Rep_name (fst typedef_info),abs_type --> rep_type) *)
-      val Abs_MT = Const(#Abs_name (fst typedef_info),rep_type --> abs_type)
+lemma call_rule:
+  fixes globals_f1 globals_f2 and x1::"'x1::prog_type pattern" and x2::"'x2::prog_type pattern" and y1 y2 A B P Q
+  assumes "set(vars_proc_global f1) \<subseteq> set globals_f1"
+  assumes "set(vars_proc_global f2) \<subseteq> set globals_f2"
+  assumes "rhoare P
+              (callproc (variable_pattern res) f1 (var_expression args))
+              (callproc (variable_pattern res) f2 (var_expression args))
+              Q"
+  defines "QB == (\<lambda>m1 m2. (\<forall>gL gR xL xR. Q (memory_update (memory_update_untyped_pattern m1 (list_pattern_untyped globals_f1) gL) res xL) 
+                       (memory_update (memory_update_untyped_pattern m2 (list_pattern_untyped globals_f2)  gL) res xR)
+                \<longrightarrow> B (memory_update_pattern (memory_update_untyped_pattern m1 (list_pattern_untyped globals_f1) gL) x1 xL) 
+                      (memory_update_pattern (memory_update_untyped_pattern m2 (list_pattern_untyped globals_f2) gL) x2 xR)))"
+  defines "C == (\<lambda>m1 m2. P (memory_update m1 args (e_fun y1 m1)) (memory_update m2 args (e_fun y2 m2)) \<and> QB m1 m2)"
+  assumes "rhoare A p1 p2 C"
+  shows "rhoare A (seq p1 (callproc x1 f1 y1)) (seq p2 (callproc x2 f2 y2)) B"
+proof -
+  def x1e == "undefined::'x1 expression" def x2e == "undefined::'x2 expression" (* TODO *)
+  def P' == "\<lambda>m1 m2. P (memory_update m1 args (e_fun y1 m1)) (memory_update m2 args (e_fun y2 m2))"
+  def Q' == "\<lambda>m1 m2. Q (memory_update m1 res (e_fun x1e m1)) (memory_update m2 res (e_fun x2e m2))"
 
-      fun export thm = thm (* Proof_Context.export lthy lthy_start [thm] |> hd *)
+  have "obs_eq' V (callproc ?x ?p ?args)
+     (seq (seq (seq (assign (p_arg ?p) ?args) (assign_default_typed ?non_parg_locals)) (p_body ?p)) (assign ?x (p_return ?p)))"
+thm callproc_rule 
 
-      (* Declaring: instantiation ModuleType = (...)procedure_type begin ... end *)
+  have Q'_foot1: "assertion_footprint_left XXX Q'" sorry
+  have Q'_foot2: "assertion_footprint_right YYY Q'" sorry
 
-  in  lthy  end
-*}
+  have "rhoare P' (callproc x1 f1 y1) (callproc x2 f2 y2) Q'"
+    using obseq_context_empty Q'_foot1 apply (rule rhoare_left_obseq_replace[where C="\<lambda>x. x"])
+     apply (rule callproc_rule)
+     close 6 (tactic "ALLGOALS (Skip_Proof.cheat_tac @{context})") (* sorry *)
+    using obseq_context_empty Q'_foot2 apply (rule rhoare_right_obseq_replace[where C="\<lambda>x. x"])
+     apply (rule callproc_rule)
+     close 6 (tactic "ALLGOALS (Skip_Proof.cheat_tac @{context})") (* sorry *)
+    
+    find_theorems "obseq_context _ (\<lambda>x. x)" 
+thm rhoare_left_obseq_replace
+(* Proof plan: 
 
+- Show:  rhoare    P{args/y}  (callproc x=f(y))  Q{x/res}    (substitution)
+- Show:  footprint QB   disjoint of   callproc x=f(y)
+- Show:  rhoare    C=P{args/y}\<and>QB     (callproc x=f(y))   Q{res/x}\<and>QB   (frame_rule)
+- Show:  Q{res/x} \<and> QB \<Longrightarrow> Q
+- Show:  rhoare    C     (callproc x=f(y))   Q    (conseq)
+- Show:  rhoare    P     (p; callproc x=f(y))   Q    (seq with assm)
 
-ML {*
-Thm.instantiate' [SOME @{ctyp "'abs::type"}, SOME @{ctyp "'rep::procedure_functor"}] [] @{thm OFCLASS_procedure_functor_class_I}
-*}
+*)
+find_theorems assertion_footprint
+  show ?thesis sorry
+qed
 
-ML {* *}
-
-instantiation X :: procedure_functor begin
-
-(* definition "procedure_functor_type_X == \<lambda>_::X itself. procedure_functor_type (TYPE(X_rep))" *)
-(* term "procedure_functor_type_X" *)
-(* thm "procedure_functor_type_X_def" *)
-
-local_setup {* fn lthy => let
-      val pftype_bind = @{binding "procedure_functor_type_X"}
-val lthy0 = lthy
-      val ((a,(b,c)),lthy) = Local_Theory.define
-          ((pftype_bind,NoSyn), 
-           ((Thm.def_binding pftype_bind,[]),
-             @{termx "\<lambda>_::X itself. procedure_functor_type (TYPE(X_rep))"})) lthy
-val _ = @{print} a
-val _ = @{print} b
-val _ = @{print} (Thm.prop_of c)
-val glthy = lthy |> Proof_Context.theory_of |> Proof_Context.init_global
-val c' = glthy |> (fn ctx => Proof_Context.get_thm ctx "procedure_functor_type_X_def")
-val c' = glthy |> (fn ctx => Proof_Context.get_thm ctx "procedure_functor_type_X_def")
-val [c'] = Proof_Context.export lthy glthy [c]
-val _ = @{print} (Thm.prop_of c')
-in lthy end
-*}
-
-ML {* Thm.prop_of @{thm  procedure_functor_type_X_def} *}
-
-local_setup {*
-fn lthy =>
-  let
-(*   val bind = @{binding X}
-  val rep_type = @{typ X_rep}
-  val AbsF = @{term Abs_X} 
-  val RepF = @{term Rep_X}
-  val Abs_inverse = @{thm Abs_X_inverse}
-  val Rep_inverse = @{thm Rep_X_inverse} 
- *)
-  (* val abs_type = @{typ X} *)
-
-val export_target = lthy
-
-       (* Declaring: definition "procedure_functor_type_AbsType (x::('a,'b) AbsType itself) == procedure_functor_type (TYPE(RepType))" *)
-(*       val pftype_bind = @{binding "procedure_functor_type_X"}
-      val ((_,(_,pftype_def)),lthy) = Local_Theory.define
-          ((pftype_bind,NoSyn), 
-           ((Thm.def_binding pftype_bind,[]),
-             @{termx "\<lambda>_::X itself. procedure_functor_type (TYPE(X_rep))"})) lthy
- *) 
-
- val pftype_def = @{thm procedure_functor_type_X_def} 
-val _ = @{print} (Thm.prop_of pftype_def)
-
-(*       (* Declaring: definition "procedure_functor_mk_untyped_AbsType x == procedure_functor_mk_untyped (Rep x)" *)
-      val pfmkuntyped_bind = Binding.prefix_name "procedure_functor_mk_untyped_" bind
-      val ((_,(_,pfmkuntyped_def)),lthy) = Local_Theory.define
-          ((pfmkuntyped_bind,NoSyn), 
-           ((Thm.def_binding pfmkuntyped_bind,[]),
-             @{termx "\<lambda>x::?'abs_type. procedure_functor_mk_untyped (?RepF x :: ?'rep_type::procedure_functor)"})) lthy
-
-      (* Declaring: definition "procedure_functor_mk_typed'_AbsType p == Abs (procedure_functor_mk_typed' p)" *)
-      val pfmktyped_bind = Binding.prefix_name "procedure_functor_mk_typed'_" bind
-      val ((_,(_,pfmktyped_def)),lthy) = Local_Theory.define
-          ((pfmktyped_bind,NoSyn), 
-           ((Thm.def_binding pfmktyped_bind,[]),
-             @{termx "\<lambda>p. ?AbsF (procedure_functor_mk_typed' p :: ?'rep_type::procedure_functor) :: 'abs_type"})) lthy *)
-
-val _ = writeln ("pftype_def "^Thm.string_of_thm @{context} pftype_def)
-
-      val OFCLASS_I = Thm.instantiate' [NONE, SOME (Thm.ctyp_of lthy @{typ X_rep})] []
-          @{thm OFCLASS_procedure_functor_class_I}
-
-
-
-(* val _ = writeln (Thm.string_of_thm @{context} OFCLASS_I) *)
-
-      (* val export_target = Proof_Context.init_global thy *)
-val export_target = lthy |> Proof_Context.theory_of |> Proof_Context.init_global
-      fun export thm = Variable.export lthy export_target [thm] |> hd
-
-val pftype_def' = pftype_def |> export
-
-val _ = writeln "XXXyyy"
-      fun instance_tac ctx = 
-        resolve_tac ctx [OFCLASS_I] 1
-THEN print_tac ctx "xxx"
-            THEN solve_tac ctx [pftype_def'] 1
-THEN print_tac ctx "yyy"
- (*            THEN solve_tac ctx [pfmkuntyped_def] 1
-            THEN solve_tac ctx [pfmktyped_def] 1
-            THEN solve_tac ctx [Abs_inverse] 1
-            THEN solve_tac ctx [Rep_inverse] 1 *)
-
-       val lthy = Class.prove_instantiation_instance instance_tac lthy  
-in (lthy) end
-*}
-
-ML Class.prove_instantiation_instance
-ML {* Thm.prop_of @{thm procedure_functor_type_X_def} *}
-instance
-apply (rule OFCLASS_procedure_functor_class_I)
-
-
-
-
-
-
-
-
-
-instantiation X :: procedure_functor begin
-local_setup {* fn lthy =>
-loc_instantiate_type_copy_procedure_functor  lthy
-*}
-end
-
-ML {* 
-fun instantiate_type_copy_procedure_functor bind abs_type_name tparams rep_type AbsF RepF Abs_inverse Rep_inverse thy =
-  let val lthy = Class.instantiation ([@{type_name X}], [], @{sort procedure_functor}) thy
-      val (tmp,lthy) = loc_instantiate_type_copy_procedure_functor bind abs_type_name tparams rep_type AbsF RepF Abs_inverse Rep_inverse lthy
-      val thy = Local_Theory.exit_global lthy
-  in (tmp,thy) end
-      val inst_global : theory -> (thm*thm*thm)*theory = instantiate_type_copy_procedure_functor 
-          @{binding X} @{type_name X} [] @{typ X_rep}
-          @{term Abs_X} @{term Rep_X}
-          @{thm Abs_X_inverse} @{thm Rep_X_inverse}
- *}
-
-
-local_setup {* fn lthy =>                                            
-let
-
-
-
-      val (_,lthy) = Local_Theory.background_theory_result inst_global lthy
-in lthy end
-*}
-
-
-
-(* local_setup {*
-declare_module_type {name= @{binding XX}, procedures=[], type_params=[]}
-*}
- *)
-(* local_setup {*
-declare_module_type_cmd @{binding X} [] [] 
-*}
-
-module_type XX = f :: "(unit,unit)procedure"
- *)
 
 end
